Add dummy return values to hands-on-session file; Move docu into workspace

workspace/src/hands-on-session/DY.HandsOnSession.Protocol.fst
@@ -9,13 +9,19 @@ open DY.Lib.Web
 (* 1. Define and setup state *)
 
 (* 2. Implement client send request and set state function *)
-// val api_request: communication_keys_sess_ids -> principal -> principal -> traceful (option (state_id & timestamp))
-// let api_request comm_keys_ids client server =
+val api_request: communication_keys_sess_ids -> principal -> principal -> traceful (option (state_id & timestamp))
+let api_request comm_keys_ids client server =
+
+  return (Some ({the_id=0}, 0)) // TODO replace with actual values, e.g. return (Some (sid, msg_id))
 
 (* 3. Implement server function that receives the request and sends a response *)
-// val api_server: communication_keys_sess_ids -> principal -> timestamp -> traceful (option timestamp)
-// let api_server comm_keys_ids server msg_id =
+val api_server: communication_keys_sess_ids -> principal -> timestamp -> traceful (option timestamp)
+let api_server comm_keys_ids server msg_id =
+
+  return (Some 0) // TODO replace with actual values, e.g. return (Some msg_id_out)
 
 (* 4. Implement client receive response and print result function *)
-// val api_response: principal -> state_id -> timestamp -> traceful (option unit)
-// let api_response client sid msg_id =
+val api_response: principal -> state_id -> timestamp -> traceful (option unit)
+let api_response client sid msg_id =
+
+  return (Some ())
